Adding some scaffolding for EPP completeness proofs

src/Network.v
@@ -1,7 +1,9 @@
 From Qoreo Require Import Base.
+Import Base.Tactics.
 From Qoreo Require Expr Choreography.
 
 Module Label := Choreography.Label.
+Module Choreography := Choreography.Choreography.
 
 From Stdlib Require Lists.List.
 Import List.ListNotations.
@@ -114,6 +116,11 @@ Module Network.
 
       step (N, cfg) (Label.EPR A B) (N', cfg')
     .
+
+    Record WF (Actors : Actor.FSet.t) (N : Network.t) :=
+        {
+            wf_domain : forall A, Actor.FSet.In A Actors <-> Actor.Map.In A N;
+        }.
     
 End Network.
 
@@ -123,7 +130,7 @@ Definition conso {A : Type} (x : A) (xso : option (list A)) : option (list A) :=
   | Some xs => Some (x :: xs)
   end.
 
-Fixpoint epp (p : Actor.t) (c : Choreography.Choreography.t): option Process.t :=
+Fixpoint epp (p : Actor.t) (c : Choreography.t): option Process.t :=
   match c with
   | [] => Some []
   | Choreography.Insn.Send A1 e A2 x :: C =>
@@ -152,3 +159,331 @@ Fixpoint epp (p : Actor.t) (c : Choreography.Choreography.t): option Process.t :
       else epp p C
   (* | _ => None *)
 end.
+
+(*
+Inductive EPP : list Actor.t -> Choreography.t -> Network.t -> Prop :=
+| epp_empty : forall C, EPP [] C (Actor.Map.empty _)
+| epp_cons : forall A Actors C P N,
+    epp A C = Some P ->
+    EPP Actors C N ->
+    EPP (A::Actors) C (Actor.Map.add A P N).
+*)
+Inductive EPP : Actor.t -> Choreography.t -> Process.t -> Prop :=
+| EPP_nil : forall A, EPP A [] []
+| EPP_disjoint : forall A I C P,
+  ~ Actor.FSet.In A (Choreography.Insn.actors I) ->
+  EPP A C P ->
+  EPP A (I :: C) P
+
+| EPP_send : forall D A C P B e y,
+    D = A ->
+    D <> B ->
+    EPP D C P ->
+    EPP D (Choreography.Insn.Send A e B y :: C) (Insn.Send e B :: P)
+| EPP_receive : forall D B C P A e y,
+    D = B ->
+    D <> A ->
+    EPP D C P ->
+    EPP D (Choreography.Insn.Send A e B y :: C) (Insn.Receive y A :: P)
+
+| EPP_EPR_1 : forall D A B x y C P,
+    D = A ->
+    D <> B ->
+    EPP D C P ->
+    EPP D (Choreography.Insn.EPR A x B y :: C) (Insn.EPR x B :: P)
+| EPP_EPR_2 : forall D A B x y C P,
+    D <> A ->
+    D = B ->
+    EPP D C P ->
+    EPP D (Choreography.Insn.EPR A x B y :: C) (Insn.EPR y A :: P)
+
+| EPP_Let : forall D A x e C P,
+    D = A ->
+    EPP D C P ->
+    EPP D (Choreography.Insn.Let A x e :: C) (Insn.Let x e :: P)
+
+| EPP_LetBang : forall D A x e C P,
+    D = A ->
+    EPP D C P ->
+    EPP D (Choreography.Insn.LetBang A x e :: C) (Insn.LetBang x e :: P)
+
+| EPP_LetPair : forall D A x1 x2 e C P,
+    D = A ->
+    EPP D C P ->
+    EPP D (Choreography.Insn.LetPair A x1 x2 e :: C) (Insn.LetPair x1 x2 e :: P)
+.
+
+Lemma EPP_correct : forall A C P,
+    EPP A C P <-> epp A C = Some P.
+Admitted.
+
+Definition EPP_N (C : Choreography.t) (N : Network.t) : Prop :=
+    forall A PA,
+        Actor.Map.MapsTo A PA N
+        <->
+        Actor.FSet.In A (Choreography.actors C)
+        /\ EPP A C PA.
+
+(* Correctness of EPP *)
+
+Theorem soundness : forall C C' cfg cfg' l N,
+
+    Choreography.step (C, cfg) l (C', cfg') ->
+    EPP_N C N ->
+    exists N', EPP_N C'  N' /\
+               Network.step (N, cfg) l (N', cfg').
+Admitted.
+
+Require Import Stdlib.Program.Equality.
+
+
+Lemma EPP_subst_neq : forall A C P B x v,
+    A <> B ->
+    EPP A C P ->
+    EPP A (Choreography.subst B x v C) P.
+Admitted.
+
+Lemma EPP_subst_eq : forall A C P x v,
+    EPP A C P ->
+    EPP A (Choreography.subst A x v C) (Process.subst x v P).
+Admitted.
+
+(** Return the choreography C' such that C -(Send A v B y)-> C' *)
+Fixpoint step_send A B (C : Choreography.t) : Choreography.t :=
+    match C with
+    | [] => []
+    | Choreography.Insn.Send A0 v0 B0 y0 :: C' =>
+        match Actor.eq_dec A A0, Actor.eq_dec B B0 with
+        | left _, left _ => Choreography.subst B0 y0 v0 C'
+        | _, _ => Choreography.Insn.Send A0 v0 B0 y0 :: (step_send A B C')
+        end
+    | I' :: C' => I' :: step_send A B C'
+    end.
+
+Lemma step_send_complete : forall C A v y B PA PB,
+    EPP A C (Insn.Send v B :: PA) ->
+    EPP B C (Insn.Receive y A :: PB) ->
+    Expr.Val v ->
+    forall cfg,
+        Choreography.step (C, cfg) (Label.Send A v B) (step_send A B C, cfg).
+Proof.
+    induction C as [ | I C'];
+        intros A v y B PA PB HEPPA HEPPB Hval cfg.
+    { contradict HEPPA. simpl; inversion 1. }
+    inversion HEPPA; subst;
+    inversion HEPPB; subst; simpl in *;
+        autorewrite with actor_db in *.
+    * destruct I as   [ (*Send*) A0 v0 B0 y0
+                    | (*EPR*)  A0 x0 B0 y0
+                    | (*Let*)  A0 x0 e0
+                    | (*Let!*) A0 x0 e0
+                    | (*LetPair *) A0 x0 y0 e0
+      ];
+        simpl in *; autorewrite with actor_db in *.
+      + destruct (Actor.eq_dec A A0); try (subst; firstorder; fail). 
+        apply Choreography.Delay.
+        { eapply IHC'; eauto. }
+        { simpl; intros D. autorewrite with actor_db. 
+          intros [[? | ?] [? | ?]]; subst; firstorder.
+        }
+      + apply Choreography.Delay.
+        { eapply IHC'; eauto. }
+        { simpl; intros D. autorewrite with actor_db. 
+          intros [[? | ?] [? | ?]]; subst; firstorder.
+        }
+
+      + apply Choreography.Delay.
+        { eapply IHC'; eauto. }
+        { simpl; intros D. autorewrite with actor_db. 
+          intros [[? | ?] ?]; subst; firstorder.
+        }
+      + apply Choreography.Delay.
+        { eapply IHC'; eauto. }
+        { simpl; intros D. autorewrite with actor_db. 
+          intros [[? | ?] ?]; subst; firstorder.
+        }
+      + apply Choreography.Delay.
+        { eapply IHC'; eauto. }
+        { simpl; intros D. autorewrite with actor_db. 
+          intros [[? | ?] ?]; subst; firstorder.
+        }
+
+    * absurd (A=A); auto.
+    * absurd (B=B); auto.
+    
+    * repeat rewrite Actor.eq_dec_refl.
+      constructor; auto.
+Qed.
+
+Lemma step_send_EPP_A : forall A B C PA PB v y,
+    EPP A C (Insn.Send v B :: PA) ->
+    EPP B C (Insn.Receive y A :: PB) ->
+    EPP A (step_send A B C) PA.
+Admitted.
+Lemma step_send_EPP_B : forall A B C PA PB v y,
+    EPP A C (Insn.Send v B :: PA) ->
+    EPP B C (Insn.Receive y A :: PB) ->
+    EPP B (step_send A B C) PB.
+Admitted.
+Lemma step_send_EPP_other : forall C D A B PD,
+        D <> A ->
+        D <> B ->
+        EPP D (step_send A B C) PD <-> EPP D C PD.
+Proof.
+    induction C as [ | I C'];
+        intros D A B PD HDA HDB.
+    { simpl. reflexivity. }
+    simpl. split; intros H.
+    * admit.
+    *
+    destruct I as   [ (*Send*) A0 v0 B0 y0
+                    | (*EPR*)  A0 x0 B0 y0
+                    | (*Let*)  A0 x0 e0
+                    | (*Let!*) A0 x0 e0
+                    | (*LetPair *) A0 x0 y0 e0
+    ].
+Admitted.
+
+Lemma step_send_EPP_N : forall A B C PA PB y v N,
+    EPP_N C N ->
+    EPP A C (Insn.Send v B :: PA) ->
+    EPP B C (Insn.Receive y A :: PB) ->
+    EPP_N (step_send A B C) (Actor.Map.add A PA (Actor.Map.add B (Process.subst y v PB) N)).
+Proof.
+    intros A B C PA PB y v N EPPN EPPA EPPB.
+    intros D PD.
+    split; intros HIn;
+        repeat rewrite Actor.MapFacts.F.add_mapsto_iff in *.
+    * admit.
+    * destruct HIn as [HIn EPPD].
+      destruct (Actor.eq_dec A D).
+      { left. subst; split; auto.  admit. }
+      { right. split; auto. admit. }
+      (* Might need a different definition of EPP_N. *)
+Admitted.
+      
+
+(*
+Lemma send_complete : forall C A v y B PA PB,
+    EPP A C (Insn.Send v B :: PA) ->
+    EPP B C (Insn.Receive y A :: PB) ->
+    Expr.Val v ->
+    exists C', 
+        (forall cfg,
+            Choreography.step (C, cfg) (Label.Send A v B) (C', cfg))
+        /\ EPP A C' PA
+        /\ EPP B C' (Process.subst y v PB)
+        /\ forall D PD, D <> A -> D <> B -> EPP D C' PD <-> EPP D C PD.
+Proof.
+    induction C as [ | I C'];
+        intros A v y B PA PB HEPPA HEPPB Hval.
+    { contradict HEPPA. simpl; inversion 1. }
+    destruct I as   [ (*Send*) A0 v0 B0 y0
+                    | (*EPR*)  A0 x0 B0 y0
+                    | (*Let*)  A0 x0 e0
+                    | (*Let!*) A0 x0 e0
+                    | (*LetPair *) A0 x0 y0 e0
+    ].
+    * inversion HEPPA; inversion HEPPB; subst;
+        try contradiction.
+      + exists (Choreography.subst B y v C').
+        split; [ | split; [ | split]].
+        2:{ apply EPP_subst_neq; auto. }
+        2:{ apply EPP_subst_eq; auto. }
+        { constructor; auto. }
+        {
+            intros D PD HDA0 HDB0.
+        }
+
+      +  destruct (IHC' A v y B PA PB) as [C0' [IHEPPA [IHEPPB IHC0']]]; auto.
+         exists (Choreography.Insn.Send A0 v0 B0 y0 :: C0'); intros.
+         repeat split; intros.
+         { apply EPP_send_other; auto. }
+         { apply EPP_send_other; auto. }
+         {
+            apply Choreography.Delay; auto.
+            intros D.
+            rewrite Actor.FSetFacts.inter_iff.
+            simpl.
+            repeat rewrite Actor.FSetFacts.add_iff.
+            repeat rewrite Actor.FSetFacts.singleton_iff.
+            intros [[? | ?] [? | ?]]; subst; contradiction.
+         }
+    * (* TODO *)
+
+Admitted.
+*)
+
+
+(** Return the choreography C' such that C -(EPR A x B y)-> C' in the configuration cfg *)
+Fixpoint step_epr A B cfg (C : Choreography.t) : Choreography.t :=
+    match C with
+    | [] => []
+    | Choreography.Insn.EPR A0 x0 B0 y0 :: C' =>
+        match Actor.eq_dec A A0, Actor.eq_dec B B0 with
+        | left _, left _ => 
+            match Config.epr cfg with
+            | (q1,q2,cfg') =>
+                Choreography.subst A x0 (Expr.Var q1)
+                (Choreography.subst B y0 (Expr.Var q2)
+                C')
+            end
+        | _, _ =>
+            Choreography.Insn.EPR A0 x0 B0 y0 :: (step_epr A B cfg C')
+        end
+    | I' :: C' => I' :: step_epr A B cfg C'
+    end.
+
+Lemma step_epr_complete : forall C A x y B PA PB,
+    EPP A C (Insn.EPR x B :: PA) ->
+    EPP B C (Insn.EPR y A :: PB) ->
+    forall cfg q1 q2 cfg',
+        Config.epr cfg = (q1,q2,cfg') ->
+        Choreography.step (C, cfg) (Label.EPR A B) (step_epr A B cfg C, cfg').
+Admitted.
+
+Lemma step_epr_EPP_N : forall A B C PA PB x y N cfg q1 q2 cfg',
+    EPP_N C N ->
+    EPP A C (Insn.EPR x B :: PA) ->
+    EPP B C (Insn.EPR y A :: PB) ->
+    Config.epr cfg = (q1, q2, cfg') ->
+    EPP_N (step_epr A B cfg C)
+        (Actor.Map.add A (Process.subst x (Expr.Var q1) PA)
+            (Actor.Map.add B (Process.subst y (Expr.Var q2) PB) N)).
+Admitted.
+
+Theorem completeness : forall N cfg l N' cfg',
+
+    Network.step (N, cfg) l (N', cfg') ->
+
+    forall C,
+    EPP_N C N ->
+    exists C', EPP_N C' N' /\
+                Choreography.step (C, cfg) l (C', cfg').
+Proof.
+    intros N cfg l N' cfg' Hstep.
+    remember (N, cfg) as cfgN.
+    remember (N', cfg') as cfgN'.
+    generalize dependent cfg. generalize dependent cfg'.
+    induction Hstep; intros cfg0' Hcfg0' cfg0 Hcfg0 C HEPP;
+        inversion Hcfg0'; inversion Hcfg0;
+        subst; clear Hcfg0' Hcfg0.
+    
+    * (* local step *) admit.
+    * (* send *)
+      apply HEPP in H0; destruct H0 as [_ HEPPA].
+      apply HEPP in H1; destruct H1 as [_ HEPPB].
+      exists (step_send A B C).
+      split.
+      { apply step_send_EPP_N; auto. }
+      { eapply step_send_complete; eauto. }
+
+    * (* EPR *) 
+      apply HEPP in H0; destruct H0 as [_ HEPPA].
+      apply HEPP in H1; destruct H1 as [_ HEPPB].
+      exists (step_epr A B cfg0 C).
+      split.
+      { eapply step_epr_EPP_N; eauto. }
+      { eapply step_epr_complete; eauto. }
+
+Admitted.
